\documentclass{article}
\usepackage[utf8]{inputenc}
\usepackage{amsmath}
\usepackage{stix}

\title{Rules of Logarithms}
\author{Michal Å pano}
\date{November 2021}

\begin{document}

\maketitle

% GENERAL STATEMENT
\[\forall x,y \in\mathbf{R^+}, \forall a > 0 \land a \neq 1, \forall s \in\mathbf{R}:\]

% RULES OF LOGARITHMS
\begin{enumerate}
    \item \textbf{Rule 1}
    \[\log_a 1 = 0\]
    $a^0 = 1$ ... $\log_a 1 = 0$
    
    \item \textbf{Rule 2}
    \[\log_a a = 1\]
    $a^1 = a$ ... $\log_a a = 1$
    
    \item \textbf{Rule 3}
    \[a^{log_a x} = x\]
    $\log_a x = \mathscr{l}$ ... $a^\mathscr{l} = x \Rightarrow a^{\log_a x} = x$
    
    \item \textbf{Rule 4}
    \[\log_a (x.y) = \log_a x + \log_a y\]
    $x = a^{\log_a x}, y = a^{\log_a y}$ ... $(x.y) = a^{\log_a x}.a^{\log_a y}$ ... $(x.y) = a^{\log_a x + \log_a y}$;\\ \textbf{Rule 3} $\Rightarrow \log_a (x.y) = \log_a x + \log_a y$
    
    \item \textbf{Rule 5}
    \[\log_a \Big(\frac{x}{y}\Big) = \log_a x - \log_a y\]
    $x = a^{\log_a x}, y = a^{\log_a y}$ ... $\big(\frac{x}{y}\big) = \frac{a^{\log_a x}}{a^{\log_a y}}$ ... $\big(\frac{x}{y}\big) = a^{\log_a x - \log_a y}$;\\
    \textbf{Rule 3} $\Rightarrow \log_a \Big(\frac{x}{y}\Big) = \log_a x - \log_a y$
    
    \item \textbf{Rule 6}
    \[\log_a x^s = s(\log_a x)\]
    $x = a^{\log_a x}$ ... $x^s = \big({a^{log_a x}}\big)^s$ ... $x^s = a^{s(log_a x)}$; \textbf{Rule 3} $\Rightarrow \log_a x^s = s(\log_a x)$
    
    \item \textbf{Rule 7}
    \[\log_a x = \frac{\log_b x}{\log_b a}\]
    $x = a^{\log_a x}$ ... $\log_b x = \log_b a^{\log_a x}$; \textbf{Rule 6} $\Rightarrow \log_b a^{\log_a x} = \log_a x \big(\log_b a\big)$\\... $\log_b x = \log_a x \big(\log_b a\big)$ $/\div\big(\log_b a\big)$ $\Rightarrow \log_a x = \frac{\log_b x}{\log_b a}$
    
\end{enumerate}

\end{document}

